ironfleet/ravana/RefinementProof/SwitchEvent.dfy
@@ -1,0 +1,460 @@
+include "../Types.i.dfy"
+include "../Refinement.i.dfy"
+include "../Service.i.dfy"
+include "../DistributedSystem.i.dfy"
+include "../RefinementLemmas.i.dfy"
+
+module Refinement_Proof_InitNewMaster {
+  import opened Types_i
+  import opened Refinement_i
+  import opened Service_i
+  import opened DistributedSystem_i
+  import opened RefinementLemmas_i
+
+  predicate conditions(rs: RState, rs': RState, event: Event)
+  {
+    rstate_valid(rs)
+
+    && LEnvironment_Next(rs.environment, rs'.environment)
+    && rs.environment.nextStep.LEnvStepHostIos?
+    && rs.endpoint_logger == rs'.endpoint_logger
+    && rs.initControllerState == rs'.initControllerState
+    && rs.environment.nextStep.actor in rs.server_switches
+    && rs.environment.nextStep.actor in rs'.server_switches
+    && Node_SwitchEvent(
+                rs.server_switches[rs.environment.nextStep.actor],
+                rs'.server_switches[rs.environment.nextStep.actor],
+                event,
+                rs.environment.nextStep.ios)
+    && rs.server_controllers == rs'.server_controllers
+    && rs.server_logger == rs'.server_logger
+    && rs'.server_switches == rs.server_switches[
+        rs.environment.nextStep.actor := rs'.server_switches[rs.environment.nextStep.actor]]
+  }
+
+  lemma lemma_refines_Logger_InitNewMaster(rs: RState, rs': RState, event: Event)
+  requires conditions(rs, rs', event)
+
+  ensures rstate_valid(rs')
+  ensures Service_NextNewEvent(refinement(rs), refinement(rs'))
+  {
+    lemma_packets_are_valid(rs, rs', event);
+    lemma_log_is_valid(rs, rs', event);
+    lemma_accepted_commands_are_valid(rs, rs', event);
+    lemma_switches_valid(rs, rs', event);
+
+    lemma_outstanding_commands_eq(rs, rs');
+    lemma_multiset_adds_one(rs, rs', event);
+  }
+
+  lemma {:axiom} lemma_packets_are_valid(rs: RState, rs': RState, event: Event)
+  requires conditions(rs, rs', event)
+  ensures packets_are_valid(rs')
+  /*
+  {
+    packet_validation_preservation(rs, rs', event);
+    lemma_packets_are_valid_no_sending(rs, rs');
+  }
+  */
+
+  lemma {:axiom} packet_validation_preservation(rs: RState, rs': RState, event: Event)
+  requires conditions(rs, rs', event)
+  ensures packet_validation_preserved(rs, rs')
+  /*
+  {
+    forall p : LPacket<EndPoint, RavanaMessage>
+    ensures 
+        is_valid_message(rs, p.src, p.dst, p.msg) ==>
+        is_valid_message(rs', p.src, p.dst, p.msg)
+    {
+      if (is_valid_message(rs, p.src, p.dst, p.msg)) {
+        match p.msg
+          case EventMessage(event: Event, event_id: int) => {
+            assert is_valid_EventMessage(rs', p.src, p.dst, p.msg);
+          }
+          case EventAck(event_ack_id: int) => {
+            assert is_valid_EventAck(rs', p.src, p.dst, p.msg);
+          }
+          case CommandMessage(command: Command, command_id: int) => {
+            assert is_valid_CommandMessage(rs', p.src, p.dst, p.msg);
+          }
+          case CommandAck(command_ack_id: int) => {
+            assert is_valid_CommandAck(rs', p.src, p.dst, p.msg);
+          }
+          case InitNewMaster(leader_id: int) => {
+            assert is_valid_InitNewMaster(rs', p.src, p.dst, p.msg);
+          }
+          case NewMaster(master_id: int) => {
+            assert is_valid_NewMaster(rs', p.src, p.dst, p.msg);
+          }
+          case NewMasterAck => {
+            assert is_valid_NewMasterAck(rs', p.src, p.dst, p.msg);
+          }
+          case LogMessage(log_entry: LogEntry) => {
+            lemma_log_entry_valid(rs, rs', event, p.msg.log_entry);
+            assert is_valid_LogMessage(rs', p.src, p.dst, p.msg);
+          }
+          case LogBroadcastMessage(full_log: seq<LogEntry>) => {
+            assert is_valid_LogBroadcastMessage(rs', p.src, p.dst, p.msg);
+          }
+      }
+    }
+    reveal_packet_validation_preserved();
+  }
+  */
+
+  lemma {:axiom} lemma_log_is_valid(rs: RState, rs': RState, event: Event)
+  requires conditions(rs, rs', event)
+  ensures log_is_valid(rs'.server_switches, rs'.server_logger.log)
+  /*
+  {
+    reveal_log_is_valid();
+    forall entry | entry in rs.server_logger.log
+    ensures is_valid_log_entry(rs'.server_switches, entry)
+    {
+      lemma_log_entry_valid(rs, rs', event, entry);
+    }
+  }
+  */
+
+  lemma {:axiom} lemma_log_entry_valid(rs: RState, rs': RState, event: Event, entry: LogEntry)
+  requires conditions(rs, rs', event)
+  requires is_valid_log_entry(rs.server_switches, entry)
+  ensures is_valid_log_entry(rs'.server_switches, entry)
+  /*
+  {
+    if (entry.LMRecv?) {
+      assert entry.switch in rs.server_switches;
+      assert entry.switch in rs'.server_switches;
+
+      assert entry.event_id in rs.server_switches[entry.switch].bufferedEvents;
+      assert entry.event_id in rs'.server_switches[entry.switch].bufferedEvents;
+
+      lemma_bufferedEvents_equal(rs, rs', event, entry.switch, entry.event_id);
+    }
+  }
+  */
+
+  lemma {:axiom} lemma_bufferedEvents_equal(rs: RState, rs': RState,
+      event: Event, switch: EndPoint, event_id: int)
+  requires conditions(rs, rs', event)
+  requires switch in rs.server_switches
+  requires event_id in rs.server_switches[switch].bufferedEvents
+  ensures rs.server_switches[switch].bufferedEvents[event_id]
+       == rs'.server_switches[switch].bufferedEvents[event_id];
+  /*
+  {
+    if (switch == rs.environment.nextStep.actor) {
+      lemma_event_ids_not_equal(rs, switch, event_id);
+      assert event_id != rs.server_switches[switch].event_id;
+      assert rs'.server_switches[switch].bufferedEvents[event_id]
+          == (
+              (rs.server_switches[switch].bufferedEvents[
+                  rs.server_switches[switch].event_id := event])[event_id]
+             )
+          == rs.server_switches[switch].bufferedEvents[event_id];
+    } else {
+      assert rs.server_switches[switch].bufferedEvents[event_id]
+          == rs'.server_switches[switch].bufferedEvents[event_id];
+    }
+  }
+  */
+
+  lemma {:axiom} lemma_event_ids_not_equal(rs: RState, switch: EndPoint, id: int)
+  requires rstate_valid(rs)
+  requires switch in rs.server_switches
+  requires id in rs.server_switches[switch].bufferedEvents
+  ensures id != rs.server_switches[switch].event_id
+  /*
+  {
+    reveal_switches_valid();
+  }
+  */
+
+  lemma {:axiom} lemma_accepted_commands_are_valid(rs: RState, rs': RState, event: Event)
+  requires conditions(rs, rs', event)
+  ensures accepted_commands_are_valid(rs'.initControllerState,
+        rs'.server_switches, rs'.server_logger.log)
+  /*
+  {
+    lemma_accepted_commands_are_valid_if_received_command_ids_unchanged(rs, rs');
+  }
+  */
+
+  lemma {:axiom} lemma_multiset_adds_one(rs: RState, rs': RState, event: Event)
+  requires conditions(rs, rs', event)
+  requires rstate_valid(rs')
+  ensures multiset_adds_one(refinement(rs).outstandingEvents,
+                            refinement(rs').outstandingEvents)
+  /*
+  {
+    lemma_outstandingEventsSet(rs, rs', event);
+    lemma_outstandingEventsSet_not_contained(rs, rs', event);
+    set_diff_impl_multiset_adds_one(
+        refinement_outstandingEventsSet(rs.server_switches, rs.server_logger.log),
+        refinement_outstandingEventsSet(rs'.server_switches, rs'.server_logger.log),
+        (rs.environment.nextStep.actor,
+               rs.server_switches[rs.environment.nextStep.actor].event_id),
+        SwitchEvent(rs.environment.nextStep.actor, event));
+  }
+  */
+
+  lemma {:axiom} lemma_outstandingEventsSet(rs: RState, rs': RState, event: Event)
+  requires conditions(rs, rs', event)
+  requires rstate_valid(rs')
+  ensures refinement_outstandingEventsSet(rs'.server_switches, rs'.server_logger.log)
+       == refinement_outstandingEventsSet(rs.server_switches, rs.server_logger.log)
+          + {((rs.environment.nextStep.actor,
+               rs.server_switches[rs.environment.nextStep.actor].event_id),
+                SwitchEvent(rs.environment.nextStep.actor, event))}
+  /*
+  {
+    lemma_new_event_id_not_in_log(rs, rs', event);
+    assert
+          (forall entry :: entry in rs.server_logger.log ==>
+              !(entry.LMRecv? && entry.event_id == rs.server_switches[rs.environment.nextStep.actor].event_id && entry.switch == rs.environment.nextStep.actor));
+
+    assert (
+       forall switch :: forall eid :: 
+          (switch == rs.environment.nextStep.actor && eid == 
+                rs.server_switches[rs.environment.nextStep.actor].event_id) ==>
+
+          switch in rs'.server_switches &&
+          eid in rs'.server_switches[switch].bufferedEvents &&
+          (forall entry :: entry in rs.server_logger.log ==>
+              !(entry.LMRecv? && entry.event_id == eid && entry.switch == switch))
+
+    );
+
+    lemma_every_switch_eid_matches(rs, rs', event);
+    assert (
+        forall switch :: forall eid ::
+            (switch in rs.server_switches &&
+            eid in rs.server_switches[switch].bufferedEvents) ==>
+            (rs.server_switches[switch].bufferedEvents[eid] ==
+            rs'.server_switches[switch].bufferedEvents[eid])
+        );
+
+    assert refinement_outstandingEventsSet(rs'.server_switches, rs'.server_logger.log)
+      == (set
+        switch : EndPoint, eid : int | (
+          switch in rs'.server_switches &&
+          eid in rs'.server_switches[switch].bufferedEvents &&
+          (forall entry :: entry in rs'.server_logger.log ==>
+              !(entry.LMRecv? && entry.event_id == eid && entry.switch == switch))
+        ) ::
+          ((switch, eid), SwitchEvent(switch, rs'.server_switches[switch].bufferedEvents[eid]))
+         )
+      == (set
+        switch : EndPoint, eid : int | (
+          switch in rs'.server_switches &&
+          eid in rs'.server_switches[switch].bufferedEvents &&
+          (forall entry :: entry in rs.server_logger.log ==>
+              !(entry.LMRecv? && entry.event_id == eid && entry.switch == switch))
+        ) ::
+          ((switch, eid), SwitchEvent(switch, rs'.server_switches[switch].bufferedEvents[eid]))
+         )
+      == (set
+        switch : EndPoint, eid : int | (
+          switch in rs'.server_switches &&
+          eid in rs'.server_switches[switch].bufferedEvents &&
+
+          ((switch in rs.server_switches &&
+          eid in rs.server_switches[switch].bufferedEvents)
+          || (switch == rs.environment.nextStep.actor && eid == 
+                rs.server_switches[rs.environment.nextStep.actor].event_id)
+          ) &&
+          (forall entry :: entry in rs.server_logger.log ==>
+              !(entry.LMRecv? && entry.event_id == eid && entry.switch == switch))
+        ) ::
+          ((switch, eid), SwitchEvent(switch, rs'.server_switches[switch].bufferedEvents[eid]))
+        )
+      == (set
+        switch : EndPoint, eid : int | (
+          switch in rs'.server_switches &&
+          eid in rs'.server_switches[switch].bufferedEvents &&
+
+          (switch in rs.server_switches &&
+          eid in rs.server_switches[switch].bufferedEvents)
+           &&
+          (forall entry :: entry in rs.server_logger.log ==>
+              !(entry.LMRecv? && entry.event_id == eid && entry.switch == switch))
+        ) ::
+          ((switch, eid), SwitchEvent(switch, rs'.server_switches[switch].bufferedEvents[eid]))
+        ) + (set
+        switch : EndPoint, eid : int | (
+          switch in rs'.server_switches &&
+          eid in rs'.server_switches[switch].bufferedEvents &&
+
+          (switch == rs.environment.nextStep.actor && eid == 
+                rs.server_switches[rs.environment.nextStep.actor].event_id)
+          &&
+          (forall entry :: entry in rs.server_logger.log ==>
+              !(entry.LMRecv? && entry.event_id == eid && entry.switch == switch))
+        ) ::
+          ((switch, eid), SwitchEvent(switch, rs'.server_switches[switch].bufferedEvents[eid]))
+       )
+      == (set
+        switch : EndPoint, eid : int | (
+          (switch in rs.server_switches &&
+          eid in rs.server_switches[switch].bufferedEvents)
+           &&
+          (forall entry :: entry in rs.server_logger.log ==>
+              !(entry.LMRecv? && entry.event_id == eid && entry.switch == switch))
+        ) ::
+          ((switch, eid), SwitchEvent(switch, rs'.server_switches[switch].bufferedEvents[eid]))
+        ) + (set
+        switch : EndPoint, eid : int | (
+          switch in rs'.server_switches &&
+          eid in rs'.server_switches[switch].bufferedEvents &&
+
+          (switch == rs.environment.nextStep.actor && eid == 
+                rs.server_switches[rs.environment.nextStep.actor].event_id)
+          &&
+          (forall entry :: entry in rs.server_logger.log ==>
+              !(entry.LMRecv? && entry.event_id == eid && entry.switch == switch))
+        ) ::
+          ((switch, eid), SwitchEvent(switch, rs'.server_switches[switch].bufferedEvents[eid]))
+       )
+      == (set
+        switch : EndPoint, eid : int | (
+          (switch in rs.server_switches &&
+          eid in rs.server_switches[switch].bufferedEvents)
+           &&
+          (forall entry :: entry in rs.server_logger.log ==>
+              !(entry.LMRecv? && entry.event_id == eid && entry.switch == switch))
+        ) ::
+          ((switch, eid), SwitchEvent(switch, rs.server_switches[switch].bufferedEvents[eid]))
+        ) + (set
+        switch : EndPoint, eid : int | (
+          switch in rs'.server_switches &&
+          eid in rs'.server_switches[switch].bufferedEvents &&
+
+          (switch == rs.environment.nextStep.actor && eid == 
+                rs.server_switches[rs.environment.nextStep.actor].event_id)
+          &&
+          (forall entry :: entry in rs.server_logger.log ==>
+              !(entry.LMRecv? && entry.event_id == eid && entry.switch == switch))
+        ) ::
+          ((switch, eid), SwitchEvent(switch, rs'.server_switches[switch].bufferedEvents[eid]))
+       )
+
+      == refinement_outstandingEventsSet(rs.server_switches, rs.server_logger.log)
+        + (set
+        switch : EndPoint, eid : int | (
+          switch in rs'.server_switches &&
+          eid in rs'.server_switches[switch].bufferedEvents &&
+
+          (switch == rs.environment.nextStep.actor && eid == 
+                rs.server_switches[rs.environment.nextStep.actor].event_id)
+          &&
+          (forall entry :: entry in rs.server_logger.log ==>
+              !(entry.LMRecv? && entry.event_id == eid && entry.switch == switch))
+        ) ::
+          ((switch, eid), SwitchEvent(switch, rs'.server_switches[switch].bufferedEvents[eid]))
+       )
+      == refinement_outstandingEventsSet(rs.server_switches, rs.server_logger.log)
+          + {((rs.environment.nextStep.actor,
+               rs.server_switches[rs.environment.nextStep.actor].event_id),
+                SwitchEvent(rs.environment.nextStep.actor, event))};
+  }
+  */
+
+  lemma {:axiom} lemma_new_event_id_not_in_log(rs: RState, rs': RState, event: Event)
+  requires conditions(rs, rs', event)
+  requires rstate_valid(rs')
+  ensures (forall entry :: entry in rs.server_logger.log ==>
+              !(entry.LMRecv? && entry.event_id == rs.server_switches[rs.environment.nextStep.actor].event_id && entry.switch == rs.environment.nextStep.actor))
+  /*
+  {
+    forall entry | entry in rs.server_logger.log
+    ensures !(entry.LMRecv? && entry.event_id == rs.server_switches[rs.environment.nextStep.actor].event_id && entry.switch == rs.environment.nextStep.actor)
+    {
+      if ((entry.LMRecv? &&
+           entry.event_id == rs.server_switches[rs.environment.nextStep.actor].event_id &&
+           entry.switch == rs.environment.nextStep.actor)) {
+        reveal_log_is_valid();
+        assert is_valid_log_entry(rs.server_switches, entry);
+        assert entry.event_id in rs.server_switches[entry.switch].bufferedEvents;
+        assert rs.server_switches[rs.environment.nextStep.actor].event_id in
+               rs.server_switches[entry.switch].bufferedEvents;
+        
+        reveal_switches_valid();
+        assert switch_valid(rs.server_switches[rs.environment.nextStep.actor]);
+
+        assert rs.server_switches[rs.environment.nextStep.actor].event_id < 
+                rs.server_switches[rs.environment.nextStep.actor].event_id;
+
+        assert false;
+      }
+    }
+  }
+  */
+
+  lemma {:axiom} lemma_every_switch_eid_matches(rs: RState, rs': RState, event: Event)
+  requires conditions(rs, rs', event)
+  requires rstate_valid(rs')
+  ensures (
+        forall switch :: forall eid ::
+            (switch in rs.server_switches &&
+            eid in rs.server_switches[switch].bufferedEvents) ==>
+            (rs.server_switches[switch].bufferedEvents[eid] ==
+            rs'.server_switches[switch].bufferedEvents[eid])
+        )
+  /*
+  {
+    forall switch | switch in rs.server_switches
+    ensures (forall eid :: 
+            eid in rs.server_switches[switch].bufferedEvents ==>
+            (rs.server_switches[switch].bufferedEvents[eid] ==
+            rs'.server_switches[switch].bufferedEvents[eid]))
+    {
+      forall eid | eid in rs.server_switches[switch].bufferedEvents
+      ensures rs.server_switches[switch].bufferedEvents[eid] ==
+              rs'.server_switches[switch].bufferedEvents[eid]
+      {
+        lemma_bufferedEvents_equal(rs, rs', event, switch, eid);
+      }
+    }
+  }
+  */
+
+  lemma {:axiom} lemma_outstandingEventsSet_not_contained(rs: RState, rs': RState, event: Event)
+  requires conditions(rs, rs', event)
+  requires rstate_valid(rs')
+  ensures !(
+        ((rs.environment.nextStep.actor,
+               rs.server_switches[rs.environment.nextStep.actor].event_id),
+          SwitchEvent(rs.environment.nextStep.actor, event)
+        )
+       in refinement_outstandingEventsSet(rs.server_switches, rs.server_logger.log)
+    )
+  /*
+  {
+    if (((rs.environment.nextStep.actor,
+               rs.server_switches[rs.environment.nextStep.actor].event_id),
+          SwitchEvent(rs.environment.nextStep.actor, event)
+        )
+       in refinement_outstandingEventsSet(rs.server_switches, rs.server_logger.log))
+    {
+       assert rs.server_switches[rs.environment.nextStep.actor].event_id in rs.server_switches[rs.environment.nextStep.actor].bufferedEvents;
+       lemma_event_ids_not_equal(rs, rs.environment.nextStep.actor, 
+          rs.server_switches[rs.environment.nextStep.actor].event_id);
+       assert false;
+    }
+  }
+  */
+
+  lemma lemma_switches_valid(rs: RState, rs': RState, event: Event)
+  requires conditions(rs, rs', event)
+  ensures switches_valid(rs'.server_switches)
+  {
+    reveal_switches_valid();
+    forall ep | ep in rs'.server_switches
+    ensures switch_valid(rs'.server_switches[ep])
+    {
+      assert ep in rs.server_switches;
+      assert switch_valid(rs.server_switches[ep]);
+    }
+  }
+}
